\begin{answer}
    Firstly,

$$
	\begin{aligned}
\frac{\partial J(\theta)}{\partial \theta_j} &= -\frac{1}{m}\sum_{i=1}^m y^{(i)} (1-g(\theta^T x^{(i)}))x^{(i)}_j + (1-y^{(i)}) (-g(\theta^T x^{(i)})) x^{(i)}_j \\
    &=  -\frac{1}{m}\sum_{i=1}^m (y^{(i)}-g(\theta^T x^{(i)})) x^{(i)}_j
	\end{aligned}

	\begin{aligned}
\therefore	
\frac{\partial J(\theta)}{\partial \theta_j} &= -\frac{1}{m}\sum_{i=1}^m y^{(i)} (1-g(\theta^T x^{(i)}))x^{(i)}_j + (1-y^{(i)}) (-g(\theta^T x^{(i)})) x^{(i)}_j \\
    &=  -\frac{1}{m}\sum_{i=1}^m (y^{(i)}-g(\theta^T x^{(i)})) x^{(i)}_j
	\end{aligned}
$$
	
And thus, for any $z$, 
$$
    \begin{aligned}
z^THz &= \frac{1}{m}\sum_{i=1}^m \sum_{j, k=1}^mg(\theta^Tx^{(i)})(1 - g(\theta^Tx^{(i)}))x_j^{(i)}x_k{^{(i)}} z_j z_k\\
        &= \frac{1}{m}\sum_{i=1}^m \sum_{j, k=1}^mg(\theta^Tx^{(i)})(1 - g(\theta^Tx^{(i)}))((x^{(i)})^Tz)^2 \ge 0
    \end{aligned}
$$
\end{answer}
