\begin{answer}

Notice 
$$
l = \sum_{i=1}^m \log p(x^{(i)}|y^{(i)}) + \log p(y^{(i)})
=\sum_{i=1}^m -\log(\sigma\sqrt(2\pi)) - \frac{(x^{(i)}-\mu_{y^{(i)}})^2}{2\sigma^2} + \log p(y^{(i)})
$$
thus,
    \[
\begin{aligned}
\frac{\partial l}{\partial \phi} &= \sum_{i=1}^m \mathbbm{1}(y^{(i)}=1)\frac{1}{\phi} +\mathbbm{1}(y^{(i)}=0)\frac{1}{1- \phi} = 0\\
& \therefore \hat{\phi} = \frac{1}{m} \sum_{i=1}^m \mathbbm{1}(y^{(i)}=1)\\
\newline
\frac{\partial l}{\partial \mu_0} &= \sum_{i=1}^m \mathbbm{1}(y^{(i)}=0)\frac{\partial}{\partial \mu_0}( -\frac{1}{2\sigma^2}(x^{(i)}-\mu_0)^2) = 0\\
&= \sum_{i=1}^m \mathbbm{1}(y^{(i)}=0)(x^{(i)}-\mu_0) = 0\\
& \therefore \hat{\mu_0} =\frac{\sum_{i=1}^m \mathbbm{1}(y^{(i)}=0)x^{(i)}}{\sum_{i=1}^m \mathbbm{1}(y^{(i)}=0)} \\
& \mbox{ similarly } \hat{\mu_1} =\frac{\sum_{i=1}^m \mathbbm{1}(y^{(i)}=1)x^{(i)}}{\sum_{i=1}^m \mathbbm{1}(y^{(i)}=1)} \\
\newline
\frac{\partial l}{\partial \sigma^2} &= \sum_{i=1}^m -\frac{1}{2\sigma^2}+\frac{(x^{(i)}-\mu_{y^{(i)}})^2}{2\sigma^4} = 0\\
& \sum_{i=1}^m \frac{\sigma^2}{2} = \sum_{i=1}^m \frac{(x^{(i)}-\mu_{y^{(i)}})^2}{2} \\
& \therefore \hat{\sigma^2} =\sum_{i=1}^m (x^{(i)}-\mu_{y^{(i)}})^2\\
\end{aligned}
    \]
\end{answer}

