\begin{answer}

$$
\begin{aligned}
p(y=1|x; \phi, \mu_0, \mu_1, \Sigma) &= \frac{p(x|y=1; \phi, \mu_0, \mu_1, \Sigma) p(y=1)}{\sum_j  p(x|y=j; \phi, \mu_0, \mu_1, \Sigma) p(y=j)}\\
&= \frac{\exp\left(-\frac{1}{2}(x-\mu_{1})^T \Sigma^{-1} (x-\mu_{1})\right)\ \phi}{ \exp\left(-\frac{1}{2}(x-\mu_{0})^T \Sigma^{-1} (x-\mu_{0})\right)\phi + \exp\left(-\frac{1}{2}(x-\mu_{0})^T \Sigma^{-1} (x-\mu_{0})\right)(1-\phi)} \\
\mbox{divide by top}&= \frac{1}{1 + \exp(-\frac{1}{2}\big[(x-\mu_{0})^T \Sigma^{-1} (x-\mu_{0})-(x-\mu_{1})^T \Sigma^{-1} (x-\mu_{1}) \big])\frac{1-\phi}{\phi}} \\
&= \frac{1}{1 + \exp(-\frac{1}{2}\big[(x-\mu_{0})^T \Sigma^{-1} (x-\mu_{0})-(x-\mu_{1})^T \Sigma^{-1} (x-\mu_{1}) \big]+ln(\frac{1-\phi}{\phi}))} \\
&= \frac{1}{1 + \exp(-\frac{1}{2}\big[ (\mu_1-\mu_0)^T \Sigma^{-1} (\mu_1-\mu_0) + 2 (\mu_1-\mu_0)^T \Sigma^{-1} x \big]+ln(\frac{1-\phi}{\phi}))} 
\end{aligned}
$$
Therefore, $\theta_0 =-\frac{1}{2}\mu_1^T \Sigma^{-1} \mu_1 + \mu_0^T \Sigma^{-1} \mu_0 - ln(\frac{1-\phi}{\phi})$; $\theta = (\mu_1-\mu_0)^T \Sigma^{-1}  $
\end{answer}
